Added three different and complementary decision procedures for classes of word problems. It would be possible to have a more sophisticated one that combines some of these capacities, but for now we just have:
        1. WORD_RULE

        This is for cases where we are effectively just arguing by
        arithmetic modulo the wordsize in the style of INT_RING. For
        example:

            WORD_RULE
              `!x y. word_add (word_neg x) y = word 0
                     ==> word_add x (word_neg y) = word 0`;;

        2. WORD_BITWISE_RULE / WORD_BITWISE_TAC

        This is for cases where we are more or less just doing
        bitwise propositional reasoning (it doesn't work with
        shifts, though with a bit more effort it could be extended),
        e.g.

            WORD_BITWISE_RULE
             `!x y z:N word.
                   word_xor x y = z /\
                   word_or (word_xor x y) (word_xor z z) = word 0
                   ==> z = word 0`;;

        3. WORD_ARITH / WORD_ARITH_TAC

        These are for cases where the reasoning is effectively linear
        arithmetic, including signed or unsigned values, e.g. this
        standard trick for doing range tests with one compare using
        precomputed constants:

            WORD_ARITH
             `!a b x:N word.
                word_ilt a b
                ==> (word_ilt a x /\ word_ilt x b <=>
                     word_ult (word_sub x (word_add a (word 1)))
                              (word_add b (word_not a)))`;;

Added definitions of more word concepts: C-style conditionals, joining and
selecting subwords, zero and sign extension (or also contraction, despite
the name):

        word_cand
        word_cor
        word_join
        word_subword
        word_sx
        word_zx

Added various new theorems about both the newly added and existing concepts;
in many cases these are just 1-liners using the decision procedures but it's
nice not to have to keep regenerating them:

        BIT_WORD_ADD
        BIT_WORD_ADD_CLAUSES
        BIT_WORD_CAND
        BIT_WORD_COR
        BIT_WORD_JOIN
        BIT_WORD_NEG
        BIT_WORD_NEG_CLAUSES
        BIT_WORD_SUB
        BIT_WORD_SUBWORD
        BIT_WORD_SUB_CLAUSES
        IVAL_WORD_AND_MASK
        IVAL_WORD_NOT
        IVAL_WORD_SX
        LE_VAL_MOD_STEP
        LT_VAL_MOD_STEP
        VAL_WORD_ADD_AND_OR
        VAL_WORD_ADD_AND_XOR
        VAL_WORD_AND_MASK
        VAL_WORD_AND_MASK_WORD
        VAL_WORD_CAND
        VAL_WORD_COR
        VAL_WORD_JOIN
        VAL_WORD_JOIN_SIMPLE
        VAL_WORD_OR_AND_XOR
        VAL_WORD_OR_DISJOINT
        VAL_WORD_ROL
        VAL_WORD_ROR
        VAL_WORD_SUBWORD
        VAL_WORD_ZX
        VAL_WORD_ZX_GEN
        WORD_ADD_0
        WORD_ADD_AC
        WORD_ADD_ASSOC
        WORD_ADD_OR
        WORD_ADD_OR_GEN
        WORD_ADD_SYM
        WORD_ADD_XOR
        WORD_ADD_XOR_GEN
        WORD_AND_0
        WORD_AND_1
        WORD_AND_NOT0
        WORD_AND_REFL
        WORD_AND_SYM
        WORD_BITMASK
        WORD_BITVAL_NOT
        WORD_CAND
        WORD_CAND_EQ_0
        WORD_CAND_NE_0
        WORD_COR
        WORD_COR_EQ_0
        WORD_COR_NE_0
        WORD_MUL_0
        WORD_MUL_AC
        WORD_MUL_ASSOC
        WORD_MUL_SYM
        WORD_NEG_0
        WORD_NEG_EQ_0
        WORD_NOT_ADD
        WORD_NOT_NEG
        WORD_NOT_SUB
        WORD_OR_0
        WORD_OR_EQ_0
        WORD_OR_NOT0
        WORD_OR_REFL
        WORD_OR_SYM
        WORD_OR_XOR
        WORD_OR_XOR_GEN
        WORD_SHL_AND
        WORD_SHL_OR
        WORD_SHL_XOR
        WORD_SUBWORD_0
        WORD_SUBWORD_JOIN_SELF
        WORD_SUB_0
        WORD_SUB_EQ_0
        WORD_SUB_LZERO
        WORD_SUB_REFL
        WORD_SX_0
        WORD_SX_SX
        WORD_USHR_AND
        WORD_USHR_OR
        WORD_USHR_XOR
        WORD_XOR_0
        WORD_XOR_EQ_0
        WORD_XOR_INT_MIN
        WORD_XOR_NOT0
        WORD_XOR_REFL
        WORD_XOR_SYM
        WORD_ZX_0
        WORD_ZX_1
        WORD_ZX_ZX

Library/words.ml
@@ -14,6 +14,12 @@
 (* for explicitness we don't overload the usual operators. Some have signed  *)
 (* and unsigned variants (e.g. `word_ushr` is unsigned/logical shift right,  *)
 (* while `word_ishr` is signed/arithmetical shift right).                    *)
+(*                                                                           *)
+(* Some simple decision procedures for proving basic equalities are here too *)
+(* and have limited and somewhat complementary scopes:                       *)
+(*  - WORD_RULE for simple algebraic properties                              *)
+(*  - WORD_BITWISE_RULE for bitwise-type properties of logical operations    *)
+(*  - WORD_ARITH for things involving numerical values                       *)
 (* ========================================================================= *)
 
 let HAS_SIZE_8 = HAS_SIZE_DIMINDEX_RULE `:8`;;
@@ -1234,6 +1240,27 @@ let BIT_WORD_XOR_ALT = prove
  (`!(x:N word) y k. bit k (word_xor x y) <=> ~(bit k x <=> bit k y)`,
   MESON_TAC[BIT_WORD_XOR; BIT_TRIVIAL; NOT_LT]);;
 
+let VAL_WORD_ADD_AND_XOR,VAL_WORD_ADD_AND_OR = (CONJ_PAIR o prove)
+ (`(!x y:N word. val x + val y = 2 * val(word_and x y) + val(word_xor x y)) /\
+   (!x y:N word. val x + val y = val(word_and x y) + val(word_or x y))`,
+  REPEAT STRIP_TAC THEN REWRITE_TAC[val_def; GSYM NSUM_LMUL] THEN
+  SIMP_TAC[GSYM NSUM_ADD; FINITE_NUMSEG_LT] THEN MATCH_MP_TAC NSUM_EQ THEN
+  REWRITE_TAC[IN_ELIM_THM; BIT_WORD_AND; BIT_WORD_XOR; BIT_WORD_OR] THEN
+  X_GEN_TAC `i:num` THEN DISCH_TAC THEN ASM_REWRITE_TAC[] THEN
+  MAP_EVERY ASM_CASES_TAC [`bit i (x:N word)`; `bit i (y:N word)`] THEN
+  ASM_REWRITE_TAC[BITVAL_CLAUSES] THEN ARITH_TAC);;
+
+let VAL_WORD_OR_DISJOINT = prove
+ (`!x y:N word.
+        word_and x y = word 0 ==> val(word_or x y) = val x + val y`,
+  REPEAT STRIP_TAC THEN ONCE_REWRITE_TAC[VAL_WORD_ADD_AND_OR] THEN
+  ASM_REWRITE_TAC[VAL_WORD_0; ADD_CLAUSES]);;
+
+let VAL_WORD_OR_AND_XOR = prove
+ (`!x y:N word. val(word_or x y) = val(word_and x y) + val(word_xor x y)`,
+  ONCE_REWRITE_TAC[ARITH_RULE `a = b + c <=> b + a = 2 * b + c`] THEN
+  MESON_TAC[VAL_WORD_ADD_AND_XOR; VAL_WORD_ADD_AND_OR]);;
+
 let word_add = new_definition
  `word_add = modular (+)`;;
 
@@ -1941,6 +1968,37 @@ let WORD_ROL_COMPOSE = prove
   REWRITE_TAC[INT_OF_NUM_ADD; GSYM num_congruent; CONG] THEN
   CONV_TAC MOD_DOWN_CONV THEN REFL_TAC);;
 
+let VAL_WORD_ROR = prove
+ (`!(w:N word) k.
+     k <= dimindex(:N)
+     ==> val(word_ror w k) =
+         2 EXP (dimindex(:N) - k) * val w MOD 2 EXP k + val w DIV 2 EXP k`,
+  REPEAT STRIP_TAC THEN
+  GEN_REWRITE_TAC RAND_CONV [ADD_SYM] THEN
+  ASM_SIMP_TAC[WORD_ROR_SHIFTS] THEN
+  W(MP_TAC o PART_MATCH (lhand o rand) VAL_WORD_OR_DISJOINT o lhand o snd) THEN
+  ANTS_TAC THENL
+   [REWRITE_TAC[WORD_EQ_BITS_ALT] THEN
+    SIMP_TAC[BIT_WORD_AND; BIT_WORD_USHR; BIT_WORD_SHL; BIT_WORD_0] THEN
+    REPEAT STRIP_TAC THEN
+    REPEAT(FIRST_X_ASSUM(MP_TAC o MATCH_MP(MESON[BIT_TRIVIAL; NOT_LE]
+     `bit i (w:N word) ==> i < dimindex(:N)`))) THEN
+    ASM_ARITH_TAC;
+    DISCH_THEN SUBST1_TAC] THEN
+  REWRITE_TAC[VAL_WORD_USHR; VAL_WORD_SHL] THEN AP_TERM_TAC THEN
+  REWRITE_TAC[GSYM MOD_MULT2; GSYM EXP_ADD] THEN
+  AP_TERM_TAC THEN AP_TERM_TAC THEN ASM_ARITH_TAC);;
+
+let VAL_WORD_ROL = prove
+ (`!(w:N word) k.
+        k <= dimindex(:N)
+        ==> val(word_rol w k) =
+            2 EXP k * val w MOD 2 EXP (dimindex(:N) - k) +
+            val w DIV 2 EXP (dimindex(:N) - k)`,
+  REPEAT STRIP_TAC THEN ASM_SIMP_TAC[WORD_ROL_ROR] THEN
+  SIMP_TAC[VAL_WORD_ROR; ARITH_RULE `n - m:num <= n`] THEN
+  ASM_SIMP_TAC[ARITH_RULE `k:num <= n ==> n - (n - k) = k`]);;
+
 let word_ule = new_definition `word_ule = relational2 (<=)`;;
 let word_uge = new_definition `word_uge = relational2 (>=)`;;
 let word_ult = new_definition `word_ult = relational2 (<)`;;
@@ -1950,3 +2008,827 @@ let word_ile = new_definition `word_ile = irelational2 (<=)`;;
 let word_ige = new_definition `word_ige = irelational2 (>=)`;;
 let word_ilt = new_definition `word_ilt = irelational2 (<)`;;
 let word_igt = new_definition `word_igt = irelational2 (>)`;;
+
+(* ------------------------------------------------------------------------- *)
+(* Simple "propagate signed value modulo" decision procedure.                *)
+(* ------------------------------------------------------------------------- *)
+
+let WORD_RULE =
+  let IVAL_WORD_ADD_REM = prove
+   (`!x y:N word.
+          ival(word_add x y) rem (&2 pow dimindex(:N)) =
+          ((ival x rem (&2 pow dimindex(:N))) +
+           (ival y rem (&2 pow dimindex(:N)))) rem (&2 pow dimindex(:N))`,
+    REWRITE_TAC[INT_ADD_REM] THEN REWRITE_TAC[INT_REM_EQ; ICONG_WORD_ADD])
+  and IVAL_WORD_SUB_REM = prove
+   (`!x y:N word.
+          ival(word_sub x y) rem (&2 pow dimindex(:N)) =
+          ((ival x rem (&2 pow dimindex(:N))) -
+           (ival y rem (&2 pow dimindex(:N)))) rem (&2 pow dimindex(:N))`,
+    REWRITE_TAC[INT_SUB_REM] THEN REWRITE_TAC[INT_REM_EQ; ICONG_WORD_SUB])
+  and IVAL_WORD_NEG_REM = prove
+   (`!x:N word.
+          ival(word_neg x) rem (&2 pow dimindex(:N)) =
+          (--(ival x rem (&2 pow dimindex(:N)))) rem (&2 pow dimindex(:N))`,
+    REWRITE_TAC[INT_NEG_REM] THEN REWRITE_TAC[INT_REM_EQ; ICONG_WORD_NEG])
+  and IVAL_WORD_MUL_REM = prove
+   (`!x y:N word.
+          ival(word_mul x y) rem (&2 pow dimindex(:N)) =
+          ((ival x rem (&2 pow dimindex(:N))) *
+           (ival y rem (&2 pow dimindex(:N)))) rem (&2 pow dimindex(:N))`,
+    REWRITE_TAC[INT_MUL_REM] THEN REWRITE_TAC[INT_REM_EQ; ICONG_WORD_MUL])
+  and IVAL_IWORD_REM = prove
+   (`!x. ival(iword x:N word) rem (&2 pow dimindex(:N)) =
+         x rem (&2 pow dimindex(:N))`,
+    REWRITE_TAC[INT_REM_EQ; IVAL_IWORD_CONG])
+  and IVAL_WORD_REM = prove
+   (`!n. ival(word n:N word) rem (&2 pow dimindex(:N)) =
+         &n rem (&2 pow dimindex(:N))`,
+    REWRITE_TAC[WORD_IWORD; INT_REM_EQ; IVAL_IWORD_CONG])
+  and IVAL_WORD_SHL_REM = prove
+   (`!(x:N word) n.
+      ival(word_shl x n) rem (&2 pow dimindex(:N)) =
+      (&2 pow n * ival x rem (&2 pow dimindex(:N))) rem (&2 pow dimindex(:N))`,
+    CONV_TAC INT_REM_DOWN_CONV THEN REWRITE_TAC[INT_REM_EQ; ICONG_WORD_SHL])
+  and INT_OF_NUM_REM = prove
+   (`&(x + y) rem (&2 pow dimindex(:N)) =
+     (&x rem (&2 pow dimindex(:N)) +
+      &y rem (&2 pow dimindex(:N))) rem (&2 pow dimindex(:N)) /\
+     &(x * y) rem (&2 pow dimindex(:N)) =
+     (&x rem (&2 pow dimindex(:N)) *
+      &y rem (&2 pow dimindex(:N))) rem (&2 pow dimindex(:N))`,
+    REWRITE_TAC[GSYM INT_OF_NUM_ADD; GSYM INT_OF_NUM_MUL] THEN
+    CONV_TAC INT_REM_DOWN_CONV THEN REWRITE_TAC[])
+  and INT_OF_NUM_VAL_REM = prove
+   (`!x:N word. &(val x) rem (&2 pow dimindex(:N)) =
+                ival x rem (&2 pow dimindex(:N))`,
+    REWRITE_TAC[REWRITE_RULE[GSYM INT_REM_EQ] IVAL_VAL_CONG])
+  and pth = prove
+   (`!v w:N word.
+          v = w <=>
+          ival v rem (&2 pow dimindex(:N)) = ival w rem (&2 pow dimindex(:N))`,
+    REWRITE_TAC[INT_REM_EQ; IVAL_CONG]) in
+  let WORD_VAL_EQ_CONV =
+    GEN_REWRITE_CONV I [pth] THENC
+    GEN_REWRITE_CONV TOP_DEPTH_CONV [WORD_NOT_AS_SUB] THENC
+    GEN_REWRITE_CONV (BINOP_CONV o TOP_DEPTH_CONV)
+     [IVAL_WORD_NEG_REM; IVAL_WORD_ADD_REM; IVAL_WORD_SUB_REM;
+      IVAL_WORD_MUL_REM; IVAL_IWORD_REM; IVAL_WORD_REM;
+      IVAL_WORD_SHL_REM; INT_OF_NUM_REM; INT_OF_NUM_VAL_REM] THENC
+    INT_REM_DOWN_CONV THENC
+    GEN_REWRITE_CONV I [INT_REM_EQ] in
+  fun tm ->
+    let avs,bod = strip_forall tm in
+    let th = ONCE_DEPTH_CONV WORD_VAL_EQ_CONV bod in
+    GENL avs (EQT_ELIM(TRANS th (EQT_INTRO(NUMBER_RULE (rand(concl th))))));;
+
+(* ------------------------------------------------------------------------- *)
+(* A somewhat complementary purely bitwise decision procedure.               *)
+(* ------------------------------------------------------------------------- *)
+
+let WORD_BITWISE_TAC =
+  let WORD_BITWISE_CONV =
+    GEN_REWRITE_CONV I [WORD_EQ_BITS_ALT] THENC
+    GEN_REWRITE_CONV (BINDER_CONV o RAND_CONV o BINOP_CONV o TOP_DEPTH_CONV)
+     [BIT_WORD_NOT; BIT_WORD_AND; BIT_WORD_OR;
+      BIT_WORD_XOR; BIT_WORD_OF_BITS; BIT_WORD_0;
+      IN_INSERT; NOT_IN_EMPTY; IN_UNIV] in
+  REPEAT GEN_TAC THEN
+  CONV_TAC(ONCE_DEPTH_CONV WORD_BITWISE_CONV) THEN
+  GEN_REWRITE_TAC DEPTH_CONV
+   [MESON[] `(!i. i < dimindex(:N) ==> P i) /\
+             (!i. i < dimindex(:N) ==> Q i) <=>
+             (!i. i < dimindex(:N) ==> P i /\ Q i)`] THEN
+  TRY(MATCH_MP_TAC(MESON[]
+       `(!i. i < dimindex(:N) ==> P i ==> Q i)
+        ==> (!i. i < dimindex(:N) ==> P i)
+             ==> (!i. i < dimindex(:N) ==> Q i)`) ORELSE
+      MATCH_MP_TAC(MESON[]
+       `(!i. i < dimindex(:N) ==> (P i <=> Q i))
+        ==> ((!i. i < dimindex(:N) ==> P i) <=>
+             (!i. i < dimindex(:N) ==> Q i))`)) THEN
+  TRY(GEN_TAC THEN DISCH_TAC) THEN ASM_REWRITE_TAC[] THEN
+  CONV_TAC TAUT;;
+
+let WORD_BITWISE_RULE tm = prove(tm,WORD_BITWISE_TAC);;
+
+(* ------------------------------------------------------------------------- *)
+(* Slightly ad hoc but useful reduction to linear arithmetic.                *)
+(* ------------------------------------------------------------------------- *)
+
+let WORD_ARITH_TAC =
+  let wordy tm =
+    match tm with Var(_,Tyapp("word",[_])) -> true | _ -> false in
+  REPEAT GEN_TAC THEN REWRITE_TAC[WORD_NOT_AS_SUB] THEN
+  REWRITE_TAC[WORD_RULE `word_shl (x:N word) 1 = word_add x x`] THEN
+  REWRITE_TAC[word_ile; word_ule; word_ilt; word_ult;
+              word_ige; word_uge; word_igt; word_ugt] THEN
+  REWRITE_TAC[irelational2; relational2; GSYM VAL_EQ] THEN
+  W(MAP_EVERY (MP_TAC o C ISPEC INT_VAL_BOUND) o find_terms wordy o snd) THEN
+  REWRITE_TAC[GSYM INT_OF_NUM_EQ; GSYM INT_OF_NUM_LE; GSYM INT_OF_NUM_LT;
+              GSYM INT_OF_NUM_GE; GSYM INT_OF_NUM_GT] THEN
+  REWRITE_TAC[INT_IVAL; INT_VAL_WORD_NEG_CASES; INT_VAL_WORD_ADD_CASES;
+              INT_VAL_WORD_SUB_CASES; VAL_WORD_0; VAL_WORD_1] THEN
+  REWRITE_TAC[TWICE_MSB] THEN INT_ARITH_TAC;;
+
+let WORD_ARITH tm = prove(tm,WORD_ARITH_TAC);;
+
+(* ------------------------------------------------------------------------- *)
+(* Zero extension and sign extension (also works for shortening modulo).     *)
+(* ------------------------------------------------------------------------- *)
+
+let word_zx = new_definition
+ `(word_zx:(M)word->(N)word) w = word(val w)`;;
+
+let VAL_WORD_ZX_GEN = prove
+ (`!x. val((word_zx:(M)word->(N)word) x) = val x MOD 2 EXP dimindex(:N)`,
+  GEN_TAC THEN REWRITE_TAC[word_zx; VAL_WORD]);;
+
+let VAL_WORD_ZX = prove
+ (`!x. dimindex(:M) <= dimindex(:N)
+       ==> val((word_zx:(M)word->(N)word) x) = val x`,
+  REPEAT STRIP_TAC THEN REWRITE_TAC[VAL_WORD_ZX_GEN] THEN
+  MATCH_MP_TAC MOD_LT THEN
+  TRANS_TAC LTE_TRANS `2 EXP dimindex(:M)` THEN
+  ASM_REWRITE_TAC[LE_EXP; VAL_BOUND] THEN
+  CONV_TAC NUM_REDUCE_CONV);;
+
+let WORD_ZX_ZX = prove
+ (`!w. dimindex(:M) <= dimindex(:N)
+       ==> (word_zx:N word->M word) ((word_zx:M word->N word) x) = x`,
+  REPEAT STRIP_TAC THEN
+  REWRITE_TAC[GSYM VAL_EQ; VAL_WORD_ZX_GEN; MOD_MOD_EXP_MIN] THEN
+  ASM_SIMP_TAC[ARITH_RULE `m <= n ==> MIN n m = m`] THEN
+  REWRITE_TAC[VAL_MOD_REFL]);;
+
+let WORD_ZX_0 = prove
+ (`(word_zx:M word->N word) (word 0) = word 0`,
+  REWRITE_TAC[GSYM VAL_EQ; VAL_WORD_ZX_GEN; VAL_WORD_0; MOD_0]);;
+
+let WORD_ZX_1 = prove
+ (`(word_zx:M word->N word) (word 1) = word 1`,
+  REWRITE_TAC[GSYM VAL_EQ; VAL_WORD_ZX_GEN; VAL_WORD_1; MOD_EQ_SELF] THEN
+  DISJ2_TAC THEN REWRITE_TAC[ARITH_RULE `1 < n <=> 2 EXP 1 <= n`] THEN
+  REWRITE_TAC[LE_EXP; DIMINDEX_GE_1; DIMINDEX_NONZERO] THEN ARITH_TAC);;
+
+let word_sx = new_definition
+ `(word_sx:(M)word->(N)word) w = iword(ival w)`;;
+
+let IVAL_WORD_SX = prove
+ (`!x. dimindex(:M) <= dimindex(:N)
+       ==> ival((word_sx:(M)word->(N)word) x) = ival x`,
+  REPEAT STRIP_TAC THEN REWRITE_TAC[IVAL_IWORD; word_sx] THEN
+  MATCH_MP_TAC IVAL_IWORD THEN
+  MP_TAC(ISPEC `x:M word` IVAL_BOUND) THEN
+  MATCH_MP_TAC(INT_ARITH
+   `m:int <= n ==> --m <= x /\ x < m ==> --n <= x /\ x < n`) THEN
+  MATCH_MP_TAC INT_POW_MONO THEN CONV_TAC INT_REDUCE_CONV THEN
+  ASM_ARITH_TAC);;
+
+let WORD_SX_SX = prove
+ (`!x. dimindex(:M) <= dimindex(:N)
+       ==> (word_sx:N word->M word) ((word_sx:M word->N word) x) = x`,
+  REPEAT STRIP_TAC THEN REWRITE_TAC[GSYM IVAL_EQ] THEN
+  ONCE_REWRITE_TAC[word_sx] THEN ASM_SIMP_TAC[IVAL_WORD_SX; IWORD_IVAL]);;
+
+let WORD_SX_0 = prove
+ (`(word_sx:M word->N word) (word 0) = word 0`,
+  REWRITE_TAC[GSYM IVAL_EQ; word_sx; IVAL_WORD_0; GSYM WORD_IWORD]);;
+
+(* ------------------------------------------------------------------------- *)
+(* Conditional AND and OR, with semantics of C's "&&" and "||"               *)
+(* ------------------------------------------------------------------------- *)
+
+let word_cand = new_definition
+ `(word_cand:N word->N word->N word) x y =
+        if ~(x = word 0) /\ ~(y = word 0) then word 1 else word 0`;;
+
+let word_cor = new_definition
+ `(word_cor:N word->N word->N word) x y =
+        if ~(x = word 0) \/ ~(y = word 0) then word 1 else word 0`;;
+
+let WORD_CAND = prove
+ (`!x y:N word.
+        word_cand x y = if x = word 0 \/ y = word 0 then word 0 else word 1`,
+  REWRITE_TAC[word_cand] THEN MESON_TAC[]);;
+
+let WORD_COR = prove
+ (`!x y:N word.
+        word_cor x y = if x = word 0 /\ y = word 0 then word 0 else word 1`,
+  REWRITE_TAC[word_cor] THEN MESON_TAC[]);;
+
+let WORD_CAND_NE_0 = prove
+ (`!x y:N word.
+        ~(word_cand x y = word 0) <=> ~(x = word 0) /\ ~(y = word 0)`,
+  REWRITE_TAC[word_cand] THEN MESON_TAC[WORD_NE_10]);;
+
+let WORD_COR_NE_0 = prove
+ (`!x y:N word.
+        ~(word_cor x y = word 0) <=> ~(x = word 0) \/ ~(y = word 0)`,
+  REWRITE_TAC[word_cor] THEN MESON_TAC[WORD_NE_10]);;
+
+let WORD_CAND_EQ_0 = prove
+ (`!x y:N word.
+        word_cand x y = word 0 <=> x = word 0 \/ y = word 0`,
+  REWRITE_TAC[word_cand] THEN MESON_TAC[WORD_NE_10]);;
+
+let WORD_COR_EQ_0 = prove
+ (`!x y:N word.
+        word_cor x y = word 0 <=> x = word 0 /\ y = word 0`,
+  REWRITE_TAC[word_cor] THEN MESON_TAC[WORD_NE_10]);;
+
+let VAL_WORD_CAND = prove
+ (`!x y:N word.
+        val(word_cand x y) =
+        if ~(val x = 0) /\ ~(val y = 0) then 1 else 0`,
+  REPEAT GEN_TAC THEN REWRITE_TAC[word_cand; VAL_EQ_0] THEN
+  COND_CASES_TAC THEN ASM_REWRITE_TAC[VAL_WORD_0; VAL_WORD_1]);;
+
+let VAL_WORD_COR = prove
+ (`!x y:N word.
+        val(word_cor x y) =
+        if ~(val x = 0) \/ ~(val y = 0) then 1 else 0`,
+  REPEAT GEN_TAC THEN REWRITE_TAC[word_cor; VAL_EQ_0] THEN
+  COND_CASES_TAC THEN ASM_REWRITE_TAC[VAL_WORD_0; VAL_WORD_1]);;
+
+let BIT_WORD_CAND = prove
+ (`!i x y:N word.
+        bit i (word_cand x y) <=> i = 0 /\ ~(x = word 0) /\ ~(y = word 0)`,
+  REPEAT GEN_TAC THEN REWRITE_TAC[word_cand] THEN
+  COND_CASES_TAC THEN ASM_REWRITE_TAC[BIT_WORD_0; BIT_WORD_1]);;
+
+let BIT_WORD_COR = prove
+ (`!i x y:N word.
+        bit i (word_cor x y) <=> i = 0 /\ (~(x = word 0) \/ ~(y = word 0))`,
+  REPEAT GEN_TAC THEN REWRITE_TAC[word_cor] THEN
+  COND_CASES_TAC THEN ASM_REWRITE_TAC[BIT_WORD_0; BIT_WORD_1]);;
+
+(* ------------------------------------------------------------------------- *)
+(* Joining, in a somewhat (over?) general sense; v is the high part, w low.  *)
+(* ------------------------------------------------------------------------- *)
+
+let word_join = new_definition
+ `(word_join:(M)word->(N)word->(P)word) v w =
+        word(2 EXP dimindex(:N) * val v + val w)`;;
+
+let VAL_WORD_JOIN = prove
+ (`!v w. val((word_join:(M)word->(N)word->(P)word) v w) =
+         (2 EXP dimindex(:N) * val v + val w) MOD 2 EXP dimindex(:P)`,
+  REWRITE_TAC[word_join; VAL_WORD]);;
+
+let BIT_WORD_JOIN = prove
+ (`!v w i.
+        bit i ((word_join:(M)word->(N)word->(P)word) v w) <=>
+        i < dimindex(:P) /\
+        (if i < dimindex(:N) then bit i w else bit (i - dimindex(:N)) v)`,
+  REPEAT GEN_TAC THEN ASM_CASES_TAC `i < dimindex(:P)` THEN
+  ASM_SIMP_TAC[BIT_TRIVIAL; GSYM NOT_LT] THEN
+  REWRITE_TAC[word_join; BIT_WORD] THEN ASM_REWRITE_TAC[BIT_VAL] THEN
+  COND_CASES_TAC THEN REWRITE_TAC[] THENL
+   [REWRITE_TAC[ODD_MOD] THEN AP_THM_TAC THEN AP_TERM_TAC THEN
+    REWRITE_TAC[DIV_MOD] THEN AP_THM_TAC THEN AP_TERM_TAC THEN
+    REWRITE_TAC[GSYM CONG] THEN MATCH_MP_TAC(NUMBER_RULE
+     `d divides e ==> (e * v + w:num == w) (mod d)`) THEN
+    ONCE_REWRITE_TAC[MULT_SYM] THEN REWRITE_TAC[GSYM(CONJUNCT2 EXP)] THEN
+    UNDISCH_TAC `i < dimindex(:N)` THEN
+    SIMP_TAC[LT_EXISTS; LEFT_IMP_EXISTS_THM] THEN
+    REWRITE_TAC[ARITH_RULE `i + SUC d = SUC i + d`] THEN
+    REWRITE_TAC[EXP_ADD; NUMBER_RULE `(a:num) divides a * b`];
+    AP_TERM_TAC THEN
+    SUBGOAL_THEN `2 EXP i = 2 EXP (dimindex(:N) + i - dimindex(:N))`
+    SUBST1_TAC THENL [AP_TERM_TAC THEN ASM_ARITH_TAC; SIMP_TAC[EXP_ADD]] THEN
+    REWRITE_TAC[GSYM DIV_DIV] THEN ONCE_REWRITE_TAC[MULT_SYM] THEN
+    SIMP_TAC[DIV_MULT_ADD; EXP_EQ_0; ARITH_EQ] THEN
+    SIMP_TAC[DIV_LT; VAL_BOUND; ADD_CLAUSES]]);;
+
+let VAL_WORD_JOIN_SIMPLE = prove
+ (`!v w.
+        dimindex(:M) + dimindex(:N) = dimindex(:P)
+        ==> val((word_join:(M)word->(N)word->(P)word) v w) =
+            2 EXP dimindex(:N) * val v + val w`,
+  REPEAT STRIP_TAC THEN REWRITE_TAC[VAL_WORD_JOIN] THEN
+  MATCH_MP_TAC MOD_LT THEN FIRST_X_ASSUM(SUBST1_TAC o SYM) THEN
+  TRANS_TAC LTE_TRANS
+   `2 EXP dimindex(:N) * (2 EXP dimindex(:M) - 1) + 2 EXP dimindex(:N)` THEN
+  CONJ_TAC THENL
+   [MATCH_MP_TAC LET_ADD2 THEN REWRITE_TAC[VAL_BOUND; LE_MULT_LCANCEL] THEN
+    DISJ2_TAC THEN MATCH_MP_TAC(ARITH_RULE `a < b ==> a <= b - 1`) THEN
+    REWRITE_TAC[VAL_BOUND];
+    REWRITE_TAC[LEFT_SUB_DISTRIB; EXP_ADD] THEN MATCH_MP_TAC(ARITH_RULE
+     `n * 1 <= n * m ==> n * m - n * 1 + n <= m * n`) THEN
+    REWRITE_TAC[LE_MULT_LCANCEL; ARITH_RULE `1 <= n <=> ~(n = 0)`] THEN
+    REWRITE_TAC[EXP_EQ_0; ARITH_EQ]]);;
+
+(* ------------------------------------------------------------------------- *)
+(* Subwords, where the (pos,len) argument is (lsb_position,length)           *)
+(* ------------------------------------------------------------------------- *)
+
+let word_subword = new_definition
+ `word_subword (w:M word) (pos,len):N word =
+        word((val w DIV (2 EXP pos)) MOD (2 EXP len))`;;
+
+let VAL_WORD_SUBWORD = prove
+ (`!pos len w:M word.
+        val(word_subword w (pos,len):N word) =
+        (val w DIV (2 EXP pos)) MOD (2 EXP (MIN len (dimindex(:N))))`,
+  REWRITE_TAC[word_subword; VAL_WORD; MOD_MOD_EXP_MIN]);;
+
+let BIT_WORD_SUBWORD = prove
+ (`!pos len (w:M word) i.
+        bit i (word_subword w (pos,len):N word) <=>
+        i < MIN len (dimindex(:N)) /\ bit (pos + i) w`,
+  REPEAT GEN_TAC THEN
+  REWRITE_TAC[ARITH_RULE `m < MIN p q <=> m < p /\ m < q`] THEN
+  ASM_CASES_TAC `i < dimindex(:N)` THEN
+  ASM_SIMP_TAC[GSYM NOT_LT; BIT_TRIVIAL] THEN
+  ASM_REWRITE_TAC[word_subword; BIT_WORD] THEN
+  REWRITE_TAC[DIV_MOD; GSYM EXP_ADD; BIT_VAL; DIV_DIV] THEN
+  ASM_CASES_TAC `i:num < len` THEN ASM_REWRITE_TAC[] THENL
+   [UNDISCH_TAC `i:num < len` THEN
+    SIMP_TAC[LT_EXISTS; LEFT_IMP_EXISTS_THM] THEN
+    X_GEN_TAC `d:num` THEN DISCH_THEN SUBST1_TAC THEN
+    REWRITE_TAC[ADD_ASSOC] THEN
+    SPEC_TAC(`pos + i:num`,`j:num`) THEN REWRITE_TAC[EXP_ADD] THEN
+    REWRITE_TAC[GSYM DIV_MOD; ODD_MOD_POW2; NOT_SUC];
+    MATCH_MP_TAC(MESON[ODD] `n = 0 ==> ~ODD n`) THEN
+    SIMP_TAC[DIV_EQ_0; EXP_EQ_0; ARITH_EQ] THEN
+    TRANS_TAC LTE_TRANS `2 EXP (pos + len)` THEN
+    SIMP_TAC[MOD_LT_EQ; EXP_EQ_0; ARITH_EQ; LE_EXP] THEN
+    ASM_ARITH_TAC]);;
+
+let WORD_SUBWORD_0 = prove
+ (`!pos len. word_subword (word 0) (pos,len) = word 0`,
+  REWRITE_TAC[word_subword; VAL_WORD_0; DIV_0; MOD_0]);;
+
+let WORD_SUBWORD_JOIN_SELF = prove
+ (`!(w:N word) k.
+        k <= dimindex(:N)
+        ==> word_subword (word_join w w:(N tybit0)word) (k,dimindex(:N)) =
+            word_ror w k`,
+  REPEAT STRIP_TAC THEN
+  REWRITE_TAC[WORD_EQ_BITS_ALT; BIT_WORD_SUBWORD; BIT_WORD_JOIN; BIT_WORD_ROR;
+              DIMINDEX_TYBIT0; ARITH_RULE `MIN n n = n`] THEN
+  X_GEN_TAC `i:num` THEN DISCH_TAC THEN
+  FIRST_ASSUM(DISJ_CASES_THEN2 SUBST1_TAC ASSUME_TAC o MATCH_MP (ARITH_RULE
+   `k:num <= n ==> k = n \/ k < n`)) THEN
+  ASM_SIMP_TAC[MOD_REFL; MOD_LT; ADD_CLAUSES;
+               ARITH_RULE `(n + i) - n:num = i`;
+               ARITH_RULE `~(n + i:num < n)`;
+               ARITH_RULE `i < n ==> n + i < 2 * n`] THEN
+  REWRITE_TAC[ADD_SYM; TAUT `(p /\ q <=> q) <=> q ==> p`] THEN
+  DISCH_THEN(K ALL_TAC) THEN ASM_ARITH_TAC);;
+
+(* ------------------------------------------------------------------------- *)
+(* Bit recursion equations for "linear" operations.                          *)
+(* ------------------------------------------------------------------------- *)
+
+let BIT_WORD_ADD = prove
+ (`!x (y:N word) i.
+        bit i (word_add x y) <=>
+        i < dimindex(:N) /\
+        ((bit i x <=> bit i y) <=>
+         ~(i = 0) /\
+         (bit (i - 1) x /\ bit (i - 1) y \/
+          (bit (i - 1) x \/ bit (i - 1) y) /\
+          ~(bit (i - 1) (word_add x y))))`,
+  let lemma = prove
+   (`2 EXP i <= (2 EXP i * b + x) MOD 2 EXP (i + 1) <=>
+     (EVEN b <=> 2 EXP i <= x MOD (2 EXP (i + 1)))`,
+    SIMP_TAC[EXP_ADD; EXP_1; MOD_MULT_MOD; EXP_EQ_0; ARITH_EQ;
+             DIV_MULT_ADD; MOD_MULT_ADD] THEN
+    REWRITE_TAC[MOD_2_CASES; EVEN_ADD] THEN
+    MAP_EVERY ASM_CASES_TAC [`EVEN b`; `EVEN(x DIV 2 EXP i)`] THEN
+    ASM_REWRITE_TAC[ADD_CLAUSES; MULT_CLAUSES; LE_ADD; NOT_LE] THEN
+    SIMP_TAC[DIVISION; EXP_EQ_0; ARITH_EQ]) in
+  REPEAT GEN_TAC THEN
+  ASM_CASES_TAC `i < dimindex(:N)` THENL
+   [ASM_REWRITE_TAC[]; ASM_MESON_TAC[NOT_LT; BIT_TRIVIAL]] THEN
+  GEN_REWRITE_TAC LAND_CONV [BIT_VAL_MOD] THEN
+  GEN_REWRITE_TAC (RAND_CONV o RAND_CONV o ONCE_DEPTH_CONV) [BIT_VAL_MOD] THEN
+  ASM_REWRITE_TAC[VAL_WORD_ADD; MOD_MOD_EXP_MIN] THEN
+  GEN_REWRITE_TAC (RAND_CONV o RAND_CONV)
+    [TAUT `~p /\ q <=> ~(~p ==> ~q)`] THEN
+  ASM_SIMP_TAC[SUB_ADD; LE_1; ARITH_RULE
+    `~(k = 0) /\ k < n ==> MIN n (k - 1 + 1) = k`] THEN
+  ASM_SIMP_TAC[NOT_IMP; ARITH_RULE `k < n ==> MIN n (k + 1) = k + 1`] THEN
+  ONCE_REWRITE_TAC[GSYM MOD_ADD_MOD] THEN
+  REWRITE_TAC[VAL_MOD_STEP; lemma; ARITH_RULE
+   `(k * b + x) + (k * c + y):num = k * (b + c) + x + y`] THEN
+  BINOP_TAC THENL
+   [MAP_EVERY ASM_CASES_TAC [`bit i (x:N word)`; `bit i (y:N word)`] THEN
+    ASM_REWRITE_TAC[BITVAL_CLAUSES] THEN CONV_TAC NUM_REDUCE_CONV;
+    SIMP_TAC[EXP_ADD; EXP_1; MOD_LT; DIVISION; EXP_EQ_0; ARITH_EQ;
+             ARITH_RULE `x < n /\ y < n ==> x + y < n * 2`]] THEN
+  ASM_CASES_TAC `i = 0` THEN
+  ASM_SIMP_TAC[EXP; MOD_1; ADD_CLAUSES; CONJUNCT1 LE;
+               EXP_EQ_0; ARITH_EQ] THEN
+  SIMP_TAC[MOD_ADD_CASES; DIVISION; EXP_EQ_0; ARITH_EQ] THEN
+  REWRITE_TAC[GSYM NOT_LE] THEN
+  MAP_EVERY ABBREV_TAC
+   [`m = val(x:N word) MOD 2 EXP i`; `n = val(y:N word) MOD 2 EXP i`] THEN
+  SUBGOAL_THEN `m < 2 EXP i /\ n < 2 EXP i` MP_TAC THENL
+   [ASM_MESON_TAC[DIVISION; EXP_EQ_0; ARITH_RULE `~(2 = 0)`]; ALL_TAC] THEN
+  SUBGOAL_THEN `2 EXP i = 2 * 2 EXP(i - 1)` SUBST1_TAC THENL
+   [ASM_SIMP_TAC[GSYM(CONJUNCT2 EXP); ADD1; SUB_ADD; LE_1];
+    ABBREV_TAC `j = i - 1` THEN
+    REWRITE_TAC[COND_SWAP; NOT_LE] THEN ASM_ARITH_TAC]);;
+
+let BIT_WORD_SUB = prove
+ (`!x (y:N word) i.
+        bit i (word_sub x y) <=>
+        i < dimindex(:N) /\
+        ((bit i x <=> bit i y) <=>
+         ~(i = 0) /\
+         (~bit (i - 1) x /\ bit (i - 1) y \/
+          (~bit (i - 1) x \/ bit (i - 1) y) /\
+          bit (i - 1) (word_sub x y)))`,
+  REPEAT GEN_TAC THEN REWRITE_TAC[WORD_RULE
+   `word_sub x y:N word = word_not(word_add (word_not x) y)`] THEN
+  REWRITE_TAC[BIT_WORD_NOT] THEN
+  ASM_CASES_TAC `i < dimindex(:N)` THEN ASM_REWRITE_TAC[] THEN
+  GEN_REWRITE_TAC (LAND_CONV o RAND_CONV) [BIT_WORD_ADD] THEN
+  ASM_SIMP_TAC[BIT_WORD_NOT; ARITH_RULE `i < n ==> i - 1 < n`] THEN
+  REWRITE_TAC[TAUT `~((~p <=> q) <=> r) <=> ((p <=> q) <=> r)`]);;
+
+let BIT_WORD_NEG = prove
+ (`!(x:N word) i.
+        bit i (word_neg x) <=>
+        i < dimindex(:N) /\
+        (bit i x <=> i = 0 \/ ~bit (i - 1) x /\ ~bit (i - 1) (word_neg x))`,
+  REPEAT GEN_TAC THEN
+  REWRITE_TAC[WORD_RULE `word_neg x:N word = word_sub (word 0) x`] THEN
+  GEN_REWRITE_TAC LAND_CONV [BIT_WORD_SUB] THEN
+  REWRITE_TAC[BIT_WORD_0] THEN CONV_TAC TAUT);;
+
+let BIT_WORD_ADD_CLAUSES = prove
+ (`(!x (y:N word).
+        bit 0 (word_add x y) <=> ~(bit 0 x <=> bit 0 y)) /\
+   (!x (y:N word) i.
+        bit (i + 1) (word_add x y) <=>
+        i + 1 < dimindex(:N) /\
+        ((bit (i + 1) x <=> bit (i + 1) y) <=>
+         (bit i x /\ bit i y \/
+          (bit i x \/ bit i y) /\ ~(bit i (word_add x y)))))`,
+  REPEAT STRIP_TAC THEN
+  GEN_REWRITE_TAC LAND_CONV [BIT_WORD_ADD] THEN
+  SIMP_TAC[DIMINDEX_GE_1; LE_1; ADD_SUB; ADD_EQ_0; ARITH_EQ]);;
+
+let BIT_WORD_SUB_CLAUSES = prove
+ (`(!x (y:N word).
+        bit 0 (word_sub x y) <=> ~(bit 0 x <=> bit 0 y)) /\
+   (!x (y:N word) i.
+        bit (i + 1) (word_sub x y) <=>
+        i + 1 < dimindex(:N) /\
+        ((bit (i + 1) x <=> bit (i + 1) y) <=>
+         (~bit i x /\ bit i y \/
+          (~bit i x \/ bit i y) /\ bit i (word_sub x y))))`,
+  REPEAT STRIP_TAC THEN
+  GEN_REWRITE_TAC LAND_CONV [BIT_WORD_SUB] THEN
+  SIMP_TAC[DIMINDEX_GE_1; LE_1; ADD_SUB; ADD_EQ_0; ARITH_EQ]);;
+
+let BIT_WORD_NEG_CLAUSES = prove
+ (`(!(x:N word).
+        bit 0 (word_neg x) = bit 0 x) /\
+   (!(x:N word) i.
+        bit (i + 1) (word_neg x) <=>
+        i + 1 < dimindex(:N) /\
+        (bit (i + 1) x <=> ~bit i x /\ ~bit i (word_neg x)))`,
+  REPEAT STRIP_TAC THEN
+  GEN_REWRITE_TAC LAND_CONV [BIT_WORD_NEG] THEN
+  SIMP_TAC[DIMINDEX_GE_1; LE_1; ADD_SUB; ADD_EQ_0; ARITH_EQ]);;
+
+let LE_VAL_MOD_STEP = prove
+ (`!(x:N word) (y:N word) i.
+        (val x MOD 2 EXP (i + 1)) <= (val y MOD 2 EXP (i + 1)) <=>
+        ~bit i x /\ bit i y \/
+        (bit i x <=> bit i y) /\ val x MOD 2 EXP i <= val y MOD 2 EXP i`,
+  REPEAT GEN_TAC THEN REWRITE_TAC[VAL_MOD_STEP] THEN
+  MAP_EVERY BOOL_CASES_TAC [`bit i (x:N word)`; `bit i (y:N word)`] THEN
+  ASM_REWRITE_TAC[BITVAL_CLAUSES; ADD_CLAUSES; MULT_CLAUSES] THEN
+  REWRITE_TAC[LE_ADD_LCANCEL; NOT_LE] THEN TRY(MATCH_MP_TAC LT_IMP_LE) THEN
+  MATCH_MP_TAC(ARITH_RULE `x:num < y ==> x < y + z`) THEN
+  SIMP_TAC[DIVISION; EXP_EQ_0; ARITH_EQ]);;
+
+let LT_VAL_MOD_STEP = prove
+ (`!(x:N word) (y:N word) i.
+        (val x MOD 2 EXP (i + 1)) < (val y MOD 2 EXP (i + 1)) <=>
+        ~bit i x /\ bit i y \/
+        (bit i x <=> bit i y) /\ val x MOD 2 EXP i < val y MOD 2 EXP i`,
+  REPEAT GEN_TAC THEN REWRITE_TAC[VAL_MOD_STEP] THEN
+  MAP_EVERY BOOL_CASES_TAC [`bit i (x:N word)`; `bit i (y:N word)`] THEN
+  ASM_REWRITE_TAC[BITVAL_CLAUSES; ADD_CLAUSES; MULT_CLAUSES] THEN
+  REWRITE_TAC[LT_ADD_LCANCEL; NOT_LT] THEN TRY(MATCH_MP_TAC LT_IMP_LE) THEN
+  MATCH_MP_TAC(ARITH_RULE `x:num < y ==> x < y + z`) THEN
+  SIMP_TAC[DIVISION; EXP_EQ_0; ARITH_EQ]);;
+
+(* ------------------------------------------------------------------------- *)
+(* Miscellaneous lemmas we don't want to keep regenerating. Many of them in  *)
+(* any case need a little bit of manual effort.                              *)
+(* ------------------------------------------------------------------------- *)
+
+let WORD_ADD_0 = prove
+ (`(!x:N word. word_add x (word 0) = x) /\
+   (!x:N word. word_add (word 0) x = x)`,
+  CONV_TAC WORD_RULE);;
+
+let WORD_ADD_SYM = prove
+ (`!x y:N word. word_add x y = word_add y x`,
+  CONV_TAC WORD_RULE);;
+
+let WORD_ADD_ASSOC = prove
+ (`!x y z:N word. word_add x (word_add y z) =
+                  word_add (word_add x y) z`,
+  CONV_TAC WORD_RULE);;
+
+let WORD_ADD_AC = prove
+ (`word_add x y = word_add y x /\
+   word_add (word_add x y) z = word_add x (word_add y z) /\
+   word_add x (word_add y z) = word_add y (word_add x z)`,
+  CONV_TAC WORD_RULE);;
+
+let WORD_MUL_0 = prove
+ (`(!x:N word. word_mul x (word 0) = word 0) /\
+   (!x:N word. word_mul (word 0) x = word 0)`,
+  CONV_TAC WORD_RULE);;
+
+let WORD_MUL_SYM = prove
+ (`!x y:N word. word_mul x y = word_mul y x`,
+  CONV_TAC WORD_RULE);;
+
+let WORD_MUL_ASSOC = prove
+ (`!x y z:N word. word_mul x (word_mul y z) =
+                  word_mul (word_mul x y) z`,
+  CONV_TAC WORD_RULE);;
+
+let WORD_MUL_AC = prove
+ (`word_mul x y = word_mul y x /\
+   word_mul (word_mul x y) z = word_mul x (word_mul y z) /\
+   word_mul x (word_mul y z) = word_mul y (word_mul x z)`,
+  CONV_TAC WORD_RULE);;
+
+let WORD_SUB_0 = prove
+ (`!x:N word. word_sub x (word 0) = x`,
+  CONV_TAC WORD_RULE);;
+
+let WORD_SUB_LZERO = prove
+ (`!x:N word. word_sub (word 0) x = word_neg x`,
+  CONV_TAC WORD_RULE);;
+
+let WORD_SUB_EQ_0 = prove
+ (`!x y:N word. word_sub x y = word 0 <=> x = y`,
+  CONV_TAC WORD_RULE);;
+
+let WORD_SUB_REFL = prove
+ (`!x:N word. word_sub x x = word 0`,
+  CONV_TAC WORD_RULE);;
+
+let WORD_NEG_0 = prove
+ (`word_neg (word 0) = word 0`,
+  CONV_TAC WORD_RULE);;
+
+let WORD_NEG_EQ_0 = prove
+ (`!x:N word. word_neg x = word 0 <=> x = word 0`,
+  CONV_TAC WORD_RULE);;
+
+let WORD_AND_REFL = prove
+ (`!x:N word. word_and x x = x`,
+  CONV_TAC WORD_BITWISE_RULE);;
+
+let WORD_AND_0 = prove
+ (`(!x:N word. word_and x (word 0) = word 0) /\
+   (!x:N word. word_and (word 0) x = word 0)`,
+  CONV_TAC WORD_BITWISE_RULE);;
+
+let WORD_AND_NOT0 = prove
+ (`(!x:N word. word_and x (word_not(word 0)) = x) /\
+   (!x:N word. word_and (word_not(word 0)) x = x)`,
+  CONV_TAC WORD_BITWISE_RULE);;
+
+let WORD_AND_SYM = prove
+ (`!x y:N word. word_and x y = word_and y x`,
+  CONV_TAC WORD_BITWISE_RULE);;
+
+let WORD_OR_REFL = prove
+ (`!x:N word. word_or x x = x`,
+  CONV_TAC WORD_BITWISE_RULE);;
+
+let WORD_OR_0 = prove
+ (`(!x:N word. word_or x (word 0) = x) /\
+   (!x:N word. word_or (word 0) x = x)`,
+  CONV_TAC WORD_BITWISE_RULE);;
+
+let WORD_OR_NOT0 = prove
+ (`(!x:N word. word_or x (word_not(word 0)) = word_not(word 0)) /\
+   (!x:N word. word_or (word_not(word 0)) x = word_not(word 0))`,
+  CONV_TAC WORD_BITWISE_RULE);;
+
+let WORD_OR_SYM = prove
+ (`!x y:N word. word_or x y = word_or y x`,
+  CONV_TAC WORD_BITWISE_RULE);;
+
+let WORD_OR_EQ_0 = prove
+ (`!x y:N word. word_or x y = word 0 <=> x = word 0 /\ y = word 0`,
+  CONV_TAC WORD_BITWISE_RULE);;
+
+let WORD_XOR_EQ_0 = prove
+ (`!x y:N word. word_xor x y = word 0 <=> x = y`,
+  CONV_TAC WORD_BITWISE_RULE);;
+
+let WORD_XOR_0 = prove
+ (`(!x:N word. word_xor x (word 0) = x) /\
+   (!x:N word. word_xor (word 0) x = x)`,
+  CONV_TAC WORD_BITWISE_RULE);;
+
+let WORD_XOR_NOT0 = prove
+ (`(!x:N word. word_xor x (word_not(word 0)) = word_not x) /\
+   (!x:N word. word_xor (word_not(word 0)) x = word_not x)`,
+  CONV_TAC WORD_BITWISE_RULE);;
+
+let WORD_XOR_REFL = prove
+ (`!x:N word. word_xor x x = word 0`,
+  REWRITE_TAC[WORD_XOR_EQ_0]);;
+
+let WORD_XOR_SYM = prove
+ (`!x y:N word. word_xor x y = word_xor y x`,
+  CONV_TAC WORD_BITWISE_RULE);;
+
+let WORD_AND_1 = prove
+ (`(!x:N word. word_and x (word 1) = if bit 0 x then word 1 else word 0) /\
+   (!x:N word. word_and (word 1) x = if bit 0 x then word 1 else word 0)`,
+  REWRITE_TAC[WORD_BITWISE_RULE
+   `word_and (word 1:N word) x = word_and x (word 1)`] THEN
+  GEN_TAC THEN COND_CASES_TAC THEN
+  REWRITE_TAC[WORD_EQ_BITS; BIT_WORD_AND; BIT_WORD_1; BIT_WORD_0] THEN
+  X_GEN_TAC `i:num` THEN ASM_CASES_TAC `i = 0` THEN
+  ASM_REWRITE_TAC[BIT_WORD_0] THEN SIMP_TAC[DIMINDEX_GE_1; LE_1]);;
+
+let WORD_NOT_NEG = prove
+ (`!x:N word. word_not(word_neg x) = word_sub x (word 1)`,
+  GEN_TAC THEN REWRITE_TAC[WORD_NOT_AS_SUB] THEN
+  AP_THM_TAC THEN AP_TERM_TAC THEN CONV_TAC WORD_RULE);;
+
+let WORD_NOT_SUB = prove
+ (`!x y:N word.
+        word_not(word_sub x y) = word_add (word_not x) y`,
+  REWRITE_TAC[WORD_NOT_AS_SUB] THEN CONV_TAC WORD_RULE);;
+
+let WORD_NOT_ADD = prove
+ (`!x y:N word.
+        word_not(word_add x y) = word_add (word_not x) (word_neg y)`,
+  REWRITE_TAC[WORD_NOT_AS_SUB] THEN CONV_TAC WORD_RULE);;
+
+let WORD_SHL_AND = prove
+ (`!(v:N word) w n.
+        word_shl (word_and v w) n =
+        word_and (word_shl v n) (word_shl w n)`,
+  REPEAT GEN_TAC THEN
+  REWRITE_TAC[WORD_EQ_BITS; BIT_WORD_SHL; BIT_WORD_AND] THEN
+  X_GEN_TAC `i:num` THEN
+  ASM_CASES_TAC `bit (i - n) (v:N word)` THEN ASM_REWRITE_TAC[] THEN
+  ASM_CASES_TAC `bit (i - n) (w:N word)` THEN ASM_REWRITE_TAC[] THEN
+  ARITH_TAC);;
+
+let WORD_USHR_AND = prove
+ (`!(v:N word) w n.
+        word_ushr (word_and v w) n =
+        word_and (word_ushr v n) (word_ushr w n)`,
+  REPEAT GEN_TAC THEN
+  REWRITE_TAC[WORD_EQ_BITS; BIT_WORD_USHR; BIT_WORD_AND] THEN
+  X_GEN_TAC `i:num` THEN ASM_CASES_TAC `i + n < dimindex(:N)` THEN
+  RULE_ASSUM_TAC(REWRITE_RULE[NOT_LT]) THEN ASM_SIMP_TAC[BIT_TRIVIAL] THEN
+  ASM_CASES_TAC `i < dimindex(:N)` THEN ASM_REWRITE_TAC[] THEN ASM_ARITH_TAC);;
+
+let WORD_SHL_OR = prove
+ (`!(v:N word) w n.
+        word_shl (word_or v w) n =
+        word_or (word_shl v n) (word_shl w n)`,
+  REPEAT GEN_TAC THEN
+  REWRITE_TAC[WORD_EQ_BITS; BIT_WORD_SHL; BIT_WORD_OR] THEN
+  X_GEN_TAC `i:num` THEN
+  ASM_CASES_TAC `bit (i - n) (v:N word)` THEN ASM_REWRITE_TAC[] THEN
+  ASM_CASES_TAC `bit (i - n) (w:N word)` THEN ASM_REWRITE_TAC[] THEN
+  ARITH_TAC);;
+
+let WORD_USHR_OR = prove
+ (`!(v:N word) w n.
+        word_ushr (word_or v w) n =
+        word_or (word_ushr v n) (word_ushr w n)`,
+  REPEAT GEN_TAC THEN
+  REWRITE_TAC[WORD_EQ_BITS; BIT_WORD_USHR; BIT_WORD_OR] THEN
+  X_GEN_TAC `i:num` THEN ASM_CASES_TAC `i + n < dimindex(:N)` THEN
+  RULE_ASSUM_TAC(REWRITE_RULE[NOT_LT]) THEN ASM_SIMP_TAC[BIT_TRIVIAL] THEN
+  ASM_CASES_TAC `i < dimindex(:N)` THEN ASM_REWRITE_TAC[] THEN ASM_ARITH_TAC);;
+
+let WORD_SHL_XOR = prove
+ (`!(v:N word) w n.
+        word_shl (word_xor v w) n =
+        word_xor (word_shl v n) (word_shl w n)`,
+  REPEAT GEN_TAC THEN
+  REWRITE_TAC[WORD_EQ_BITS; BIT_WORD_SHL; BIT_WORD_XOR] THEN
+  X_GEN_TAC `i:num` THEN
+  ASM_CASES_TAC `bit (i - n) (v:N word)` THEN ASM_REWRITE_TAC[] THEN
+  ASM_CASES_TAC `bit (i - n) (w:N word)` THEN ASM_REWRITE_TAC[] THEN
+  ARITH_TAC);;
+
+let WORD_USHR_XOR = prove
+ (`!(v:N word) w n.
+        word_ushr (word_xor v w) n =
+        word_xor (word_ushr v n) (word_ushr w n)`,
+  REPEAT GEN_TAC THEN
+  REWRITE_TAC[WORD_EQ_BITS; BIT_WORD_USHR; BIT_WORD_XOR] THEN
+  X_GEN_TAC `i:num` THEN ASM_CASES_TAC `i + n < dimindex(:N)` THEN
+  RULE_ASSUM_TAC(REWRITE_RULE[NOT_LT]) THEN ASM_SIMP_TAC[BIT_TRIVIAL] THEN
+  ASM_CASES_TAC `i < dimindex(:N)` THEN ASM_REWRITE_TAC[] THEN ASM_ARITH_TAC);;
+
+let WORD_ADD_XOR_GEN = prove
+ (`!x y:N word.
+        word_add x y = word_add (word_shl (word_and x y) 1) (word_xor x y)`,
+  REPEAT GEN_TAC THEN
+  REWRITE_TAC[GSYM VAL_CONG; CONG; VAL_WORD_ADD; VAL_WORD_SHL] THEN
+  CONV_TAC MOD_DOWN_CONV THEN AP_THM_TAC THEN AP_TERM_TAC THEN
+  REWRITE_TAC[EXP_1; VAL_WORD_ADD_AND_XOR]);;
+
+let WORD_ADD_OR_GEN = prove
+ (`!x y:N word. word_add x y = word_add (word_and x y) (word_or x y)`,
+  REPEAT GEN_TAC THEN
+  REWRITE_TAC[GSYM VAL_CONG; CONG; VAL_WORD_ADD; VAL_WORD_SHL] THEN
+  CONV_TAC MOD_DOWN_CONV THEN AP_THM_TAC THEN AP_TERM_TAC THEN
+  REWRITE_TAC[GSYM VAL_WORD_ADD_AND_OR]);;
+
+let WORD_OR_XOR_GEN = prove
+ (`!x y:N word. word_or x y = word_add (word_and x y) (word_xor x y)`,
+  REPEAT GEN_TAC THEN
+  REWRITE_TAC[GSYM VAL_CONG; CONG; VAL_WORD_ADD] THEN
+  CONV_TAC MOD_DOWN_CONV THEN REWRITE_TAC[VAL_WORD_OR_AND_XOR]);;
+
+let WORD_ADD_XOR = prove
+ (`!x y:N word. word_and x y = word 0 ==> word_add x y = word_xor x y`,
+  REPEAT STRIP_TAC THEN ONCE_REWRITE_TAC[WORD_ADD_XOR_GEN] THEN
+  ASM_REWRITE_TAC[] THEN CONV_TAC WORD_RULE);;
+
+let WORD_OR_XOR = prove
+ (`!x y:N word. word_and x y = word 0 ==> word_or x y = word_xor x y`,
+  REPEAT STRIP_TAC THEN
+  ASM_REWRITE_TAC[WORD_OR_XOR_GEN] THEN CONV_TAC WORD_RULE);;
+
+let WORD_ADD_OR = prove
+ (`!x y:N word. word_and x y = word 0 ==> word_add x y = word_or x y`,
+  SIMP_TAC[WORD_OR_XOR; WORD_ADD_XOR]);;
+
+let WORD_XOR_INT_MIN = prove
+ (`!w:N word. word_xor word_INT_MIN w = word_add word_INT_MIN w`,
+  GEN_TAC THEN ONCE_REWRITE_TAC[WORD_ADD_XOR_GEN] THEN
+  REWRITE_TAC[WORD_RULE `w:N word = word_add x w <=> x = word 0`] THEN
+  REWRITE_TAC[WORD_SHL_AND] THEN
+  MATCH_MP_TAC(WORD_BITWISE_RULE `x = word 0 ==> word_and x y = word 0`) THEN
+  REWRITE_TAC[WORD_EQ_BITS; BIT_WORD_0; BIT_WORD_SHL; BIT_WORD_INT_MIN] THEN
+  ARITH_TAC);;
+
+let WORD_BITVAL_NOT = prove
+ (`!b. word(bitval(~b)) = word_sub (word 1) (word(bitval b))`,
+  GEN_TAC THEN BOOL_CASES_TAC `b:bool` THEN
+  ASM_REWRITE_TAC[BITVAL_CLAUSES] THEN CONV_TAC WORD_RULE);;
+
+let IVAL_WORD_NOT = prove
+ (`!x:N word. ival(word_not x) = --(ival x + &1)`,
+  REWRITE_TAC[IVAL_IWORD_GALOIS] THEN
+  REWRITE_TAC[INT_ARITH `--x:int <= --(y + &1) <=> y < x`] THEN
+  REWRITE_TAC[INT_ARITH `--(x + &1):int < y <=> --y <= x`] THEN
+  REWRITE_TAC[IVAL_BOUND] THEN
+  REWRITE_TAC[IWORD_INT_NEG; IWORD_INT_ADD; IWORD_IVAL; GSYM WORD_IWORD] THEN
+  CONV_TAC WORD_RULE);;
+
+(* ------------------------------------------------------------------------- *)
+(* Some lemmas about masks 000..001111..1111 and their values.               *)
+(* ------------------------------------------------------------------------- *)
+
+let VAL_WORD_AND_MASK = prove
+ (`!(x:N word) k.
+        val(word_and x (word_of_bits {i | i < k})) = val x MOD (2 EXP k)`,
+  REPEAT GEN_TAC THEN REWRITE_TAC[val_def] THEN
+  SIMP_TAC[BINARY_DIGITSUM_MOD; FINITE_NUMSEG_LT; NSUM_RESTRICT_SET] THEN
+  MATCH_MP_TAC NSUM_EQ THEN
+  REWRITE_TAC[IN_ELIM_THM; BIT_WORD_AND; IN_ELIM_THM; BIT_WORD_OF_BITS] THEN
+  REPEAT STRIP_TAC THEN ASM_REWRITE_TAC[bitval] THEN ARITH_TAC);;
+
+let IVAL_WORD_AND_MASK = prove
+ (`!(x:N word) k.
+        k < dimindex(:N)
+        ==> ival(word_and x (word_of_bits {i | i < k})) =
+            ival x rem (&2 pow k)`,
+  REPEAT STRIP_TAC THEN ASM_SIMP_TAC[INT_REM_IVAL; LT_IMP_LE] THEN
+  REWRITE_TAC[GSYM VAL_WORD_AND_MASK; ival] THEN
+  MATCH_MP_TAC(MESON[] `p ==> (if p then x else y) = x`) THEN
+  REWRITE_TAC[VAL_WORD_AND_MASK] THEN TRANS_TAC LTE_TRANS `2 EXP k` THEN
+  SIMP_TAC[DIVISION; EXP_EQ_0; ARITH_EQ; LE_EXP] THEN ASM_ARITH_TAC);;
+
+let VAL_WORD_AND_MASK_WORD = prove
+ (`!x k. val(word_and x (word(2 EXP k - 1))) = val x MOD 2 EXP k`,
+  REWRITE_TAC[GSYM WORD_OF_BITS_MASK; VAL_WORD_AND_MASK]);;
+
+let WORD_BITMASK = prove
+ (`!k. word_of_bits {i | i < k}:N word =
+       word_sub (word_of_bits {k}) (word 1)`,
+  REWRITE_TAC[WORD_OF_BITS_MASK; WORD_OF_BITS_SING_AS_WORD] THEN
+  REWRITE_TAC[WORD_SUB; ARITH_RULE `1 <= n <=> ~(n = 0)`] THEN
+  REWRITE_TAC[EXP_EQ_0; ARITH_EQ]);;
